Spectre.thy
@@ -36,7 +36,7 @@ function vote_Spectre :: "('a::linorder,'b) pre_digraph \<Rightarrow>'a \<Righta
   if ((a \<rightarrow>\<^sup>*\<^bsub>V\<^esub> c) \<and> \<not>(a \<rightarrow>\<^sup>+\<^bsub>V\<^esub> b)) then -1 else
   if ((a \<rightarrow>\<^sup>+\<^bsub>V\<^esub> b) \<and> (a \<rightarrow>\<^sup>+\<^bsub>V\<^esub> c)) then 
    (sumlist_break b c (map (\<lambda>i.
- (vote_Spectre (DAG.reduce_past V a) i b c)) (sorted_list_of_set (past_nodes V a))))
+ (vote_Spectre (reduce_past V a) i b c)) (sorted_list_of_set (past_nodes V a))))
  else 
    sumlist_break b c (map (\<lambda>i.
    (vote_Spectre V i b c)) (sorted_list_of_set (future_nodes V a))))"
@@ -51,10 +51,10 @@ next
   fix x a b c
   assume bD: " \<not> (\<not> blockDAG V \<or> a \<notin> verts V \<or> b \<notin> verts V \<or> c \<notin> verts V)"
   then have "a \<in> verts V"  by simp
-  then have "card (verts (DAG.reduce_past V a)) < card (verts V)"   
+  then have "card (verts (reduce_past V a)) < card (verts V)"   
     using bD blockDAG.reduce_less
     by metis
-  then show "((DAG.reduce_past V a, x, b, c), V, a, b, c)
+  then show "((reduce_past V a, x, b, c), V, a, b, c)
        \<in> measures
            [\<lambda>(V, a, b, c). card (verts V),
             \<lambda>(V, a, b, c). card {e. e \<rightarrow>\<^sup>*\<^bsub>V\<^esub> a}]"
@@ -137,12 +137,13 @@ lemma Spectre_theo:
   and "P 1"
   and "P (-1)" 
   and "P (sumlist_break b c (map (\<lambda>i.
- (vote_Spectre (DAG.reduce_past V a) i b c)) (sorted_list_of_set ((past_nodes V a)))))"
+ (vote_Spectre (reduce_past V a) i b c)) (sorted_list_of_set ((past_nodes V a)))))"
   and "P (sumlist_break b c (map (\<lambda>i.
    (vote_Spectre V i b c)) (sorted_list_of_set (future_nodes V a))))"
 shows "P (vote_Spectre V a b c)"
   using assms vote_Spectre.simps
-  by auto 
+  by (metis (mono_tags, lifting)) 
+  
 
 lemma domain_Spectre:
   shows "vote_Spectre V a b c \<in> {-1, 0, 1}"
@@ -151,7 +152,7 @@ proof(rule Spectre_theo)
   show "1 \<in> {- 1, 0, 1}" by simp
   show " - 1 \<in> {- 1, 0, 1}" by simp
   show "sumlist_break b c
-     (map (\<lambda>i. vote_Spectre (DAG.reduce_past V a) i b c) (sorted_list_of_set (past_nodes V a)))
+     (map (\<lambda>i. vote_Spectre (reduce_past V a) i b c) (sorted_list_of_set (past_nodes V a)))
     \<in> {- 1, 0, 1}" using domain_sumlist by simp 
   show "sumlist_break b c (map (\<lambda>i. vote_Spectre V i b c)
   (sorted_list_of_set (future_nodes V a))) \<in> {- 1, 0, 1}" using domain_sumlist by simp 
@@ -198,9 +199,9 @@ proof -
              \<not> (a \<rightarrow>\<^sup>*\<^bsub>V\<^esub> c \<and> (a, b) \<notin> (arcs_ends V)\<^sup>+) \<Longrightarrow>
              a \<rightarrow>\<^sup>+\<^bsub>V\<^esub> b \<and> a \<rightarrow>\<^sup>+\<^bsub>V\<^esub> c \<Longrightarrow>
              x \<in> set (sorted_list_of_set (past_nodes V a)) \<Longrightarrow>
-             blockDAG (DAG.reduce_past V a) \<Longrightarrow>
+             blockDAG (reduce_past V a) \<Longrightarrow>
              b \<noteq> c \<longrightarrow>
-             vote_Spectre (DAG.reduce_past V a) x b c = - vote_Spectre (DAG.reduce_past V a) x c b)
+             vote_Spectre (reduce_past V a) x b c = - vote_Spectre (reduce_past V a) x c b)
         "
         and
        "(\<And>x. \<not> (\<not> blockDAG V \<or> a \<notin> verts V \<or> b \<notin> verts V \<or> c \<notin> verts V) \<Longrightarrow>
